Remove seq_ prefixes

examples/seq/Tests.fst
@@ -39,106 +39,106 @@ open FStar.Sequence
 
 (** test1 asserts various statements that trivially follow from the ambient sequence facts **)
 private let test1 () : Lemma (True) =
-  assert (seq_length (seq_empty #int) == 0);
-  assert (forall (s: seq bool). seq_length s == 0 ==> s == seq_empty);
-  assert (forall (v: list int). seq_length (seq_singleton v) == 1);
-  assert (forall (s: seq int) (v: int). seq_length (seq_build s v) == 1 + seq_length s);
-  assert (forall (v: nat). seq_index (seq_singleton v) 0 == v);
-  assert (~(seq_contains seq_empty 42));
-  assert (forall (s: seq int). seq_take s 0 == seq_empty);
-  assert (forall (s: seq int). seq_drop s 0 == s);
+  assert (length (empty #int) == 0);
+  assert (forall (s: seq bool). length s == 0 ==> s == empty);
+  assert (forall (v: list int). length (singleton v) == 1);
+  assert (forall (s: seq int) (v: int). length (build s v) == 1 + length s);
+  assert (forall (v: nat). index (singleton v) 0 == v);
+  assert (~(contains empty 42));
+  assert (forall (s: seq int). take s 0 == empty);
+  assert (forall (s: seq int). drop s 0 == s);
   ()
 
 (** test2 builds a sequence [1; 2; 3; 4; 5] and asserts various properties about it **)
 private let test2 () : Lemma (True) =
-  let s1 = nil $:: 1 in
+  let s1 = empty $:: 1 in
   let s2 = s1 $:: 2 in
   let s3 = s2 $:: 3 in
   let s4 = s3 $:: 4 in
   let s5 = s4 $:: 5 in
-  assert (seq_length s2 = 1 + seq_length s1);
-  assert (seq_length s2 = 2);
-  assert (seq_length s5 = 5);
+  assert (length s2 = 1 + length s1);
+  assert (length s2 = 2);
+  assert (length s5 = 5);
   assert (s5 $@ 1 == 2);
   assert (forall (s: seq int) (n: nat). n < 2 ==> (s2 $+ s) $@ n = s2 $@ n);
-  assert (seq_drop (seq_drop s5 1) 2 == seq_drop s5 3);
-  assert (forall (v: int). seq_length (s5 $:: v) = 6);
+  assert (drop (drop s5 1) 2 == drop s5 3);
+  assert (forall (v: int). length (s5 $:: v) = 6);
   assert (s3 $<= s5);
-  assert (seq_length (seq_update s5 3 7) == 5);
-  assert ((seq_update s5 3 7) $@ 2 == 3);
-  assert ((seq_update s5 3 7) $@ 3 == 7);
-  assert (seq_length (seq_slice s5 1 3) == 2)
+  assert (length (update s5 3 7) == 5);
+  assert ((update s5 3 7) $@ 2 == 3);
+  assert ((update s5 3 7) $@ 3 == 7);
+  assert (length (slice s5 1 3) == 2)
 
 (** test3 establishes that appending a take and a drop with the same index produces the same sequence **)
-private let test3 (s: seq int) (n: nat{n <= seq_length s})
-  : Lemma (s $== ((seq_take s n) $+ (seq_drop s n))) =
+private let test3 (s: seq int) (n: nat{n <= length s})
+  : Lemma (s $== ((take s n) $+ (drop s n))) =
   ()
 
-(** test4 tests the use of seq_rank to establish a decreases clause **)
-private let rec test4 (s: seq int) : Tot int (decreases seq_rank s) =
-  if seq_length s = 0 then
+(** test4 tests the use of rank to establish a decreases clause **)
+private let rec test4 (s: seq int) : Tot int (decreases rank s) =
+  if length s = 0 then
     0
   else
-    1 + test4 (seq_drop s 1)
+    1 + test4 (drop s 1)
 
-(** test5 tests the use of seq_length to establish a decreases clause in a case where seq_rank won't work **)
-private let rec test5 (s: seq int) : Tot int (decreases seq_length s) =
-  if seq_length s = 0 then
+(** test5 tests the use of length to establish a decreases clause in a case where rank won't work **)
+private let rec test5 (s: seq int) : Tot int (decreases length s) =
+  if length s = 0 then
     0
   else
-    1 + test5 (seq_take s (seq_length s - 1))
+    1 + test5 (take s (length s - 1))
 
 (** test6 simply asserts all the ambient sequence facts **)
 private let test6 () : Lemma (True) =
-  assert (forall (ty: Type).{:pattern seq_empty #ty} seq_length (seq_empty #ty) = 0);
-  assert (forall (ty: Type) (s: seq ty).{:pattern seq_length s} seq_length s = 0 ==> s == seq_empty);
-  assert (forall (ty: Type) (v: ty).{:pattern seq_length (seq_singleton v)} seq_length (seq_singleton v) = 1);
-  assert (forall (ty: Type) (s: seq ty) (v: ty).{:pattern seq_build s v} seq_length (seq_build s v) = 1 + seq_length s);
-  assert (forall (ty: Type) (s0: seq ty) (s1: seq ty).{:pattern seq_length (seq_append s0 s1)}
-           seq_length (seq_append s0 s1) = seq_length s0 + seq_length s1);
-  assert (forall (ty: Type) (s: seq ty) (i: nat{i < seq_length s}) (v: ty).{:pattern seq_length (seq_update s i v)}
-           seq_length (seq_update s i v) = seq_length s);
-  assert (forall (ty: Type) (s: seq ty) (i: nat{i < seq_length s}) (v: ty) (n: nat{n < seq_length (seq_update s i v)})
-            .{:pattern seq_index (seq_update s i v) n}
-            n < seq_length s ==>
-              (i = n ==> seq_index (seq_update s i v) n == v)
-            /\ (i <> n ==> seq_index (seq_update s i v) n == seq_index s n));
-  assert (forall (ty: Type) (s: seq ty) (x: ty).{:pattern seq_contains s x}
-           seq_contains s x <==> (exists (i: nat).{:pattern seq_index s i} i < seq_length s /\ seq_index s i == x));
-  assert (forall (ty: Type) (x: ty).{:pattern seq_contains seq_empty x} ~(seq_contains seq_empty x));
-  assert (forall (ty: Type) (s: seq ty) (v: ty) (x: ty).{:pattern seq_contains (seq_build s v) x}
-            seq_contains (seq_build s v) x <==> (v == x \/ seq_contains s x));
-  assert (forall (ty: Type) (s: seq ty) (n: nat{n <= seq_length s}) (x: ty).{:pattern seq_contains (seq_take s n) x}
-            seq_contains (seq_take s n) x <==>
-            (exists (i: nat).{:pattern seq_index s i} i < n /\ i < seq_length s /\ seq_index s i == x));
-  assert (forall (ty: Type) (s: seq ty) (n: nat{n <= seq_length s}) (x: ty).{:pattern seq_contains (seq_drop s n) x}
-            seq_contains (seq_drop s n) x <==>
-            (exists (i: nat).{:pattern seq_index s i} n <= i && i < seq_length s /\ seq_index s i == x));
-  assert (forall (ty: Type) (s0: seq ty) (s1: seq ty).{:pattern seq_equal s0 s1}
-           seq_equal s0 s1 <==>
-           seq_length s0 == seq_length s1 /\
-             (forall j.{:pattern seq_index s0 j \/ seq_index s1 j}
-                0 <= j && j < seq_length s0 ==> seq_index s0 j == seq_index s1 j));
-  assert (forall (ty: Type) (a: seq ty) (b: seq ty).{:pattern seq_equal a b} seq_equal a b ==> a == b);
-  assert (forall (ty: Type) (s0: seq ty) (s1: seq ty).{:pattern seq_is_prefix s0 s1}
-            seq_is_prefix s0 s1 <==>
-              seq_length s0 <= seq_length s1
-            /\ (forall (j: nat).{:pattern seq_index s0 j \/ seq_index s1 j}
-                 j < seq_length s0 ==> seq_index s0 j == seq_index s1 j));
-  assert (forall (ty: Type) (s: seq ty) (n: nat).{:pattern seq_length (seq_take s n)}
-            n <= seq_length s ==> seq_length (seq_take s n) = n);
-  assert (forall (ty: Type) (s: seq ty) (n: nat). {:pattern seq_length (seq_drop s n)}
-            n <= seq_length s ==> seq_length (seq_drop s n) = seq_length s - n);
-  assert (forall (ty: Type) (v: ty).{:pattern seq_rank v} seq_rank v == v);
-  assert (forall (ty: Type) (s: seq ty) (i: nat).{:pattern seq_rank (seq_index s i)}
-            i < seq_length s ==> seq_rank (seq_index s i) << seq_rank s);
-  assert (forall (ty: Type) (s: seq ty) (i: nat).{:pattern seq_rank (seq_drop s i)}
-            0 < i && i <= seq_length s ==> seq_rank (seq_drop s i) << seq_rank s);
-  assert (forall (ty: Type) (s: seq ty) (i: nat).{:pattern seq_length (seq_take s i)}
-            i < seq_length s ==> seq_length (seq_take s i) << seq_length s);
-  assert (forall (ty: Type) (s: seq ty) (i: nat) (j: nat).{:pattern seq_length (seq_append (seq_take s i) (seq_drop s j))}
-            i < j && j <= seq_length s ==> seq_length (seq_append (seq_take s i) (seq_drop s j)) << seq_length s);
-  assert (forall (ty: Type) (s: seq ty) (n: nat).{:pattern seq_drop s n} n = 0 ==> seq_drop s n == s);
-  assert (forall (ty: Type) (s: seq ty) (n: nat).{:pattern seq_take s n} n = 0 ==> seq_take s n == seq_empty);
-  assert (forall (ty: Type) (s: seq ty) (m: nat) (n: nat).{:pattern seq_drop (seq_drop s m) n}
-            m + n <= seq_length s ==> seq_drop (seq_drop s m) n == seq_drop s (m + n))
+  assert (forall (ty: Type).{:pattern empty #ty} length (empty #ty) = 0);
+  assert (forall (ty: Type) (s: seq ty).{:pattern length s} length s = 0 ==> s == empty);
+  assert (forall (ty: Type) (v: ty).{:pattern length (singleton v)} length (singleton v) = 1);
+  assert (forall (ty: Type) (s: seq ty) (v: ty).{:pattern build s v} length (build s v) = 1 + length s);
+  assert (forall (ty: Type) (s0: seq ty) (s1: seq ty).{:pattern length (append s0 s1)}
+           length (append s0 s1) = length s0 + length s1);
+  assert (forall (ty: Type) (s: seq ty) (i: nat{i < length s}) (v: ty).{:pattern length (update s i v)}
+           length (update s i v) = length s);
+  assert (forall (ty: Type) (s: seq ty) (i: nat{i < length s}) (v: ty) (n: nat{n < length (update s i v)})
+            .{:pattern index (update s i v) n}
+            n < length s ==>
+              (i = n ==> index (update s i v) n == v)
+            /\ (i <> n ==> index (update s i v) n == index s n));
+  assert (forall (ty: Type) (s: seq ty) (x: ty).{:pattern contains s x}
+           contains s x <==> (exists (i: nat).{:pattern index s i} i < length s /\ index s i == x));
+  assert (forall (ty: Type) (x: ty).{:pattern contains empty x} ~(contains empty x));
+  assert (forall (ty: Type) (s: seq ty) (v: ty) (x: ty).{:pattern contains (build s v) x}
+            contains (build s v) x <==> (v == x \/ contains s x));
+  assert (forall (ty: Type) (s: seq ty) (n: nat{n <= length s}) (x: ty).{:pattern contains (take s n) x}
+            contains (take s n) x <==>
+            (exists (i: nat).{:pattern index s i} i < n /\ i < length s /\ index s i == x));
+  assert (forall (ty: Type) (s: seq ty) (n: nat{n <= length s}) (x: ty).{:pattern contains (drop s n) x}
+            contains (drop s n) x <==>
+            (exists (i: nat).{:pattern index s i} n <= i && i < length s /\ index s i == x));
+  assert (forall (ty: Type) (s0: seq ty) (s1: seq ty).{:pattern equal s0 s1}
+           equal s0 s1 <==>
+           length s0 == length s1 /\
+             (forall j.{:pattern index s0 j \/ index s1 j}
+                0 <= j && j < length s0 ==> index s0 j == index s1 j));
+  assert (forall (ty: Type) (a: seq ty) (b: seq ty).{:pattern equal a b} equal a b ==> a == b);
+  assert (forall (ty: Type) (s0: seq ty) (s1: seq ty).{:pattern is_prefix s0 s1}
+            is_prefix s0 s1 <==>
+              length s0 <= length s1
+            /\ (forall (j: nat).{:pattern index s0 j \/ index s1 j}
+                 j < length s0 ==> index s0 j == index s1 j));
+  assert (forall (ty: Type) (s: seq ty) (n: nat).{:pattern length (take s n)}
+            n <= length s ==> length (take s n) = n);
+  assert (forall (ty: Type) (s: seq ty) (n: nat). {:pattern length (drop s n)}
+            n <= length s ==> length (drop s n) = length s - n);
+  assert (forall (ty: Type) (v: ty).{:pattern rank v} rank v == v);
+  assert (forall (ty: Type) (s: seq ty) (i: nat).{:pattern rank (index s i)}
+            i < length s ==> rank (index s i) << rank s);
+  assert (forall (ty: Type) (s: seq ty) (i: nat).{:pattern rank (drop s i)}
+            0 < i && i <= length s ==> rank (drop s i) << rank s);
+  assert (forall (ty: Type) (s: seq ty) (i: nat).{:pattern length (take s i)}
+            i < length s ==> length (take s i) << length s);
+  assert (forall (ty: Type) (s: seq ty) (i: nat) (j: nat).{:pattern length (append (take s i) (drop s j))}
+            i < j && j <= length s ==> length (append (take s i) (drop s j)) << length s);
+  assert (forall (ty: Type) (s: seq ty) (n: nat).{:pattern drop s n} n = 0 ==> drop s n == s);
+  assert (forall (ty: Type) (s: seq ty) (n: nat).{:pattern take s n} n = 0 ==> take s n == empty);
+  assert (forall (ty: Type) (s: seq ty) (m: nat) (n: nat).{:pattern drop (drop s m) n}
+            m + n <= length s ==> drop (drop s m) n == drop s (m + n))
