ulib/experimental/FStar.Sequence.Base.fst
@@ -40,107 +40,107 @@ chosen as in those axioms.
 *)
 module FStar.Sequence.Base
 
-open FStar.List.Tot
+module FLT = FStar.List.Tot
 
 /// Internally, we represent a sequence as a list.
 
 type seq (ty: Type) = list ty
 
-/// We represent the Dafny function `Seq#Length` with `seq_length`:
+/// We represent the Dafny function `Seq#Length` with `length`:
 ///
 /// function Seq#Length<T>(Seq T): int;
 
-let seq_length = length
+let length = FLT.length
 
-/// We represent the Dafny function `Seq#Empty` with `seq_empty`:
+/// We represent the Dafny function `Seq#Empty` with `empty`:
 /// 
 /// function Seq#Empty<T>(): Seq T;
 
-let seq_empty (#ty: Type) : seq ty = []
+let empty (#ty: Type) : seq ty = []
 
-/// We represent the Dafny function `Seq#Singleton` with `seq_singleton`:
+/// We represent the Dafny function `Seq#Singleton` with `singleton`:
 ///
 /// function Seq#Singleton<T>(T): Seq T;
 
-let seq_singleton (#ty: Type) (v: ty) : seq ty =
+let singleton (#ty: Type) (v: ty) : seq ty =
   [v]
 
-/// We represent the Dafny function `Seq#Index` with `seq_index`:
+/// We represent the Dafny function `Seq#Index` with `index`:
 ///
 /// function Seq#Index<T>(Seq T, int): T;
 
-let seq_index (#ty: Type) (s: seq ty) (i: nat{i < seq_length s}) : ty =
-  index s i
+let index (#ty: Type) (s: seq ty) (i: nat{i < length s}) : ty =
+  FLT.index s i
 
-/// We represent the Dafny function `Seq#Build` with `seq_build`:
+/// We represent the Dafny function `Seq#Build` with `build`:
 /// 
 /// function Seq#Build<T>(s: Seq T, val: T): Seq T;
 
-let seq_build (#ty: Type) (s: seq ty) (v: ty) : seq ty =
-  append s [v]
+let build (#ty: Type) (s: seq ty) (v: ty) : seq ty =
+  FLT.append s [v]
 
-/// We represent the Dafny function `Seq#Append` with `seq_append`:
+/// We represent the Dafny function `Seq#Append` with `append`:
 ///
 /// function Seq#Append<T>(Seq T, Seq T): Seq T;
 
-let seq_append = append
+let append = FLT.append
 
-/// We represent the Dafny function `Seq#Update` with `seq_update`:
+/// We represent the Dafny function `Seq#Update` with `update`:
 ///
 /// function Seq#Update<T>(Seq T, int, T): Seq T;
 
-let seq_update (#ty: Type) (s: seq ty) (i: nat{i < seq_length s}) (v: ty) : seq ty =
-  let s1, _, s2 = split3 s i in
+let update (#ty: Type) (s: seq ty) (i: nat{i < length s}) (v: ty) : seq ty =
+  let s1, _, s2 = FLT.split3 s i in
   append s1 (append [v] s2)
 
-/// We represent the Dafny function `Seq#Contains` with `seq_contains`:
+/// We represent the Dafny function `Seq#Contains` with `contains`:
 ///
 /// function Seq#Contains<T>(Seq T, T): bool;
 
-let seq_contains (#ty: Type) (s: seq ty) (v: ty) : Type0 =
-  memP v s
+let contains (#ty: Type) (s: seq ty) (v: ty) : Type0 =
+  FLT.memP v s
 
-/// We represent the Dafny function `Seq#Take` with `seq_take`:
+/// We represent the Dafny function `Seq#Take` with `take`:
 ///
 /// function Seq#Take<T>(s: Seq T, howMany: int): Seq T;
 
-let seq_take (#ty: Type) (s: seq ty) (howMany: nat{howMany <= seq_length s}) : seq ty =
-  let result, _ = splitAt howMany s in
+let take (#ty: Type) (s: seq ty) (howMany: nat{howMany <= length s}) : seq ty =
+  let result, _ = FLT.splitAt howMany s in
   result
 
-/// We represent the Dafny function `Seq#Drop` with `seq_drop`:
+/// We represent the Dafny function `Seq#Drop` with `drop`:
 ///
 /// function Seq#Drop<T>(s: Seq T, howMany: int): Seq T;
 
-let seq_drop (#ty: Type) (s: seq ty) (howMany: nat{howMany <= seq_length s}) : seq ty =
-  let _, result = splitAt howMany s in
+let drop (#ty: Type) (s: seq ty) (howMany: nat{howMany <= length s}) : seq ty =
+  let _, result = FLT.splitAt howMany s in
   result
 
-/// We represent the Dafny function `Seq#Equal` with `seq_equal`.
+/// We represent the Dafny function `Seq#Equal` with `equal`.
 ///
 /// function Seq#Equal<T>(Seq T, Seq T): bool;
 
-let seq_equal (#ty: Type) (s0: seq ty) (s1: seq ty) : Type0 =
-  seq_length s0 == seq_length s1 /\
-    (forall j.{:pattern seq_index s0 j \/ seq_index s1 j}
-      0 <= j && j < seq_length s0 ==> seq_index s0 j == seq_index s1 j)
+let equal (#ty: Type) (s0: seq ty) (s1: seq ty) : Type0 =
+  length s0 == length s1 /\
+    (forall j.{:pattern index s0 j \/ index s1 j}
+      0 <= j && j < length s0 ==> index s0 j == index s1 j)
 
 /// Instead of representing the Dafny function `Seq#SameUntil`, which
 /// is only ever used in Dafny to represent prefix relations, we
-/// instead use `seq_is_prefix`.
+/// instead use `is_prefix`.
 ///
 /// function Seq#SameUntil<T>(Seq T, Seq T, int): bool;
 
-let seq_is_prefix (#ty: Type) (s0: seq ty) (s1: seq ty) : Type0 =
-    seq_length s0 <= seq_length s1
-  /\ (forall (j: nat).{:pattern seq_index s0 j \/ seq_index s1 j}
-     j < seq_length s0 ==> seq_index s0 j == seq_index s1 j)
+let is_prefix (#ty: Type) (s0: seq ty) (s1: seq ty) : Type0 =
+    length s0 <= length s1
+  /\ (forall (j: nat).{:pattern index s0 j \/ index s1 j}
+     j < length s0 ==> index s0 j == index s1 j)
 
-/// We represent the Dafny function `Seq#Rank` with `seq_rank`.
+/// We represent the Dafny function `Seq#Rank` with `rank`.
 ///
 /// function Seq#Rank<T>(Seq T): int;
 
-let seq_rank (#ty: Type) (v: ty) = v
+let rank (#ty: Type) (v: ty) = v
 
 /// We now prove each of the facts that comprise `all_dafny_seq_facts`.
 /// For fact `xxx_fact`, we prove it with `xxx_lemma`.  Sometimes, that
@@ -157,15 +157,15 @@ private let singleton_length_one_lemma () : Lemma (singleton_length_one_fact) =
   ()
 
 private let build_increments_length_lemma () : Lemma (build_increments_length_fact) =
-  introduce forall (ty: Type) (s: seq ty) (v: ty). seq_length (seq_build s v) = 1 + seq_length s
+  introduce forall (ty: Type) (s: seq ty) (v: ty). length (build s v) = 1 + length s
   with (
-    append_length s [v]
+    FLT.append_length s [v]
   )
 
 private let rec index_into_build_helper (#ty: Type) (s: list ty) (v: ty) (i: nat{i < length (append s [v])})
   : Lemma (requires i <= length s)
           (ensures  index (append s [v]) i == (if i = length s then v else index s i)) =
-  append_length s [v];
+  FLT.append_length s [v];
   match s with
   | [] -> ()
   | hd :: tl ->
@@ -174,17 +174,17 @@ private let rec index_into_build_helper (#ty: Type) (s: list ty) (v: ty) (i: nat
 private let index_into_build_lemma ()
   : Lemma (requires build_increments_length_fact)
           (ensures  index_into_build_fact ()) =
-  introduce forall (ty: Type) (s: seq ty) (v: ty) (i: nat{i < seq_length (seq_build s v)}).
-                (i = seq_length s ==> seq_index (seq_build s v) i == v)
-              /\ (i <> seq_length s ==> seq_index (seq_build s v) i == seq_index s i)
+  introduce forall (ty: Type) (s: seq ty) (v: ty) (i: nat{i < length (build s v)}).
+                (i = length s ==> index (build s v) i == v)
+              /\ (i <> length s ==> index (build s v) i == index s i)
   with (
     index_into_build_helper s v i
   )
 
 private let append_sums_lengths_lemma () : Lemma (append_sums_lengths_fact) =
-  introduce forall (ty: Type) (s0: seq ty) (s1: seq ty). seq_length (seq_append s0 s1) = seq_length s0 + seq_length s1
+  introduce forall (ty: Type) (s0: seq ty) (s1: seq ty). length (append s0 s1) = length s0 + length s1
   with (
-    append_length s0 s1
+    FLT.append_length s0 s1
   )
 
 private let index_into_singleton_lemma (_: squash singleton_length_one_fact) : Lemma (index_into_singleton_fact ()) =
@@ -199,9 +199,9 @@ private let rec index_after_append_helper (ty: Type) (s0: list ty) (s1: list ty)
 
 private let index_after_append_lemma (_: squash append_sums_lengths_fact) : Lemma (index_after_append_fact ()) =
   introduce
-    forall (ty: Type) (s0: seq ty) (s1: seq ty) (n: nat{n < seq_length (seq_append s0 s1)}).
-        (n < seq_length s0 ==> seq_index (seq_append s0 s1) n == seq_index s0 n)
-      /\ (seq_length s0 <= n ==> seq_index (seq_append s0 s1) n == seq_index s1 (n - seq_length s0))
+    forall (ty: Type) (s0: seq ty) (s1: seq ty) (n: nat{n < length (append s0 s1)}).
+        (n < length s0 ==> index (append s0 s1) n == index s0 n)
+      /\ (length s0 <= n ==> index (append s0 s1) n == index s1 (n - length s0))
   with (
     index_after_append_helper ty s0 s1 n
   )
@@ -209,23 +209,23 @@ private let index_after_append_lemma (_: squash append_sums_lengths_fact) : Lemm
 private let rec lemma_splitAt_fst_length (#a:Type) (n:nat) (l:list a) :
   Lemma
     (requires (n <= length l))
-    (ensures  (length (fst (splitAt n l)) = n)) =
+    (ensures  (length (fst (FLT.splitAt n l)) = n)) =
   match n, l with
   | 0, _ -> ()
   | _, [] -> ()
   | _, _ :: l' -> lemma_splitAt_fst_length (n - 1) l'
 
 private let update_maintains_length_helper (#ty: Type) (s: list ty) (i: nat{i < length s}) (v: ty)
-  : Lemma (length (seq_update s i v) = length s) =
-  let s1, _, s2 = split3 s i in
+  : Lemma (length (update s i v) = length s) =
+  let s1, _, s2 = FLT.split3 s i in
     lemma_splitAt_fst_length i s;
-    lemma_splitAt_snd_length i s;
-    append_length [v] s2;
-    append_length s1 (append [v] s2)
+    FLT.lemma_splitAt_snd_length i s;
+    FLT.append_length [v] s2;
+    FLT.append_length s1 (append [v] s2)
 
 private let update_maintains_length_lemma () : Lemma (update_maintains_length_fact) =
-  introduce forall (ty: Type) (s: seq ty) (i: nat{i < seq_length s}) (v: ty).
-    seq_length (seq_update s i v) = seq_length s
+  introduce forall (ty: Type) (s: seq ty) (i: nat{i < length s}) (v: ty).
+    length (update s i v) = length s
   with (
     update_maintains_length_helper s i v
   )
@@ -235,9 +235,9 @@ private let rec update_then_index_helper
   (s: list ty)
   (i: nat{i < length s})
   (v: ty)
-  (n: nat{n < length (seq_update s i v)})
+  (n: nat{n < length (update s i v)})
   : Lemma (requires n < length s)
-          (ensures  index (seq_update s i v) n == (if i = n then v else index s n)) =
+          (ensures  index (update s i v) n == (if i = n then v else index s n)) =
   match s with
   | hd :: tl ->
       if i = 0 || n = 0 then ()
@@ -246,10 +246,10 @@ private let rec update_then_index_helper
 private let update_then_index_lemma () : Lemma (update_then_index_fact) =
   update_maintains_length_lemma ();
   introduce
-    forall (ty: Type) (s: seq ty) (i: nat{i < seq_length s}) (v: ty) (n: nat{n < seq_length (seq_update s i v)}).
-      n < seq_length s ==>
-          (i = n ==> seq_index (seq_update s i v) n == v)
-        /\ (i <> n ==> seq_index (seq_update s i v) n == seq_index s n)
+    forall (ty: Type) (s: seq ty) (i: nat{i < length s}) (v: ty) (n: nat{n < length (update s i v)}).
+      n < length s ==>
+          (i = n ==> index (update s i v) n == v)
+        /\ (i <> n ==> index (update s i v) n == index s n)
   with
     introduce _ ==> _
     with given_antecedent. (
@@ -259,18 +259,18 @@ private let update_then_index_lemma () : Lemma (update_then_index_fact) =
 private let contains_iff_exists_index_lemma () : Lemma (contains_iff_exists_index_fact) =
   introduce 
     forall (ty: Type) (s: seq ty) (x: ty).
-      seq_contains s x <==> (exists (i: nat).{:pattern seq_index s i} i < seq_length s /\ seq_index s i == x)
+      contains s x <==> (exists (i: nat).{:pattern index s i} i < length s /\ index s i == x)
   with (
-    introduce seq_contains s x ==> (exists (i: nat).{:pattern seq_index s i} i < seq_length s /\ seq_index s i == x)
+    introduce contains s x ==> (exists (i: nat).{:pattern index s i} i < length s /\ index s i == x)
     with given_antecedent. (
-      introduce exists (i: nat). i < seq_length s /\ seq_index s i == x
-      with (index_of s x) and ()
+      introduce exists (i: nat). i < length s /\ index s i == x
+      with (FLT.index_of s x) and ()
     );
-    introduce (exists (i: nat).{:pattern seq_index s i} i < seq_length s /\ seq_index s i == x) ==> seq_contains s x
+    introduce (exists (i: nat).{:pattern index s i} i < length s /\ index s i == x) ==> contains s x
     with given_antecedent. (
-      eliminate exists (i: nat). i < seq_length s /\ seq_index s i == x
+      eliminate exists (i: nat). i < length s /\ index s i == x
       returns _
-      with _. lemma_index_memP s i
+      with _. FLT.lemma_index_memP s i
     )
   )
 
@@ -278,25 +278,25 @@ private let empty_doesnt_contain_anything_lemma () : Lemma (empty_doesnt_contain
   ()
 
 private let rec build_contains_equiv_helper (ty: Type) (s: list ty) (v: ty) (x: ty)
-  : Lemma (memP x (append s [v]) <==> (v == x \/ memP x s)) =
+  : Lemma (FLT.memP x (append s [v]) <==> (v == x \/ FLT.memP x s)) =
   match s with
   | [] -> ()
   | hd :: tl ->
      eliminate x == hd \/ ~(x == hd)
-     returns memP x (append s [v]) <==> (v == x \/ memP x s)
+     returns FLT.memP x (append s [v]) <==> (v == x \/ FLT.memP x s)
      with _. ()
      and _. build_contains_equiv_helper ty tl v x
 
 private let build_contains_equiv_lemma () : Lemma (build_contains_equiv_fact) =
   introduce 
     forall (ty: Type) (s: seq ty) (v: ty) (x: ty).
-      seq_contains (seq_build s v) x <==> (v == x \/ seq_contains s x)
+      contains (build s v) x <==> (v == x \/ contains s x)
   with (
     build_contains_equiv_helper ty s v x
   )
 
 private let rec take_contains_equiv_exists_helper1 (ty: Type) (s: list ty) (n: nat{n <= length s}) (x: ty)
-  : Lemma (requires memP x (seq_take s n))
+  : Lemma (requires FLT.memP x (take s n))
           (ensures (exists (i: nat).{:pattern index s i} i < n /\ i < length s /\ index s i == x)) =
   match s with
   | hd :: tl ->
@@ -315,22 +315,22 @@ private let rec take_contains_equiv_exists_helper1 (ty: Type) (s: list ty) (n: n
 
 private let rec take_contains_equiv_exists_helper2 (ty: Type) (s: list ty) (n: nat{n <= length s}) (x: ty) (i: nat)
   : Lemma (requires (i < n /\ i < length s /\ index s i == x))
-          (ensures  memP x (seq_take s n)) =
+          (ensures  FLT.memP x (take s n)) =
   match s with
   | hd :: tl ->
      eliminate x == hd \/ ~(x == hd)
-     returns memP x (seq_take s n)
+     returns FLT.memP x (take s n)
      with case_x_eq_hd. ()
      and case_x_ne_hd. take_contains_equiv_exists_helper2 ty tl (n - 1) x (i - 1)
 
 private let take_contains_equiv_exists_helper3 (ty: Type) (s: list ty) (n: nat{n <= length s}) (x: ty)
-  : Lemma (memP x (seq_take s n) <==>
+  : Lemma (FLT.memP x (take s n) <==>
            (exists (i: nat).{:pattern index s i} i < n /\ i < length s /\ index s i == x)) =
-  introduce memP x (seq_take s n) ==>
+  introduce FLT.memP x (take s n) ==>
               (exists (i: nat).{:pattern index s i} i < n /\ i < length s /\ index s i == x)
   with given_antecedent. (take_contains_equiv_exists_helper1 ty s n x);
   introduce (exists (i: nat).{:pattern index s i} i < n /\ i < length s /\ index s i == x) ==>
-              memP x (seq_take s n)
+              FLT.memP x (take s n)
   with given_antecedent. (
     eliminate exists (i: nat). i < n /\ i < length s /\ index s i == x
     returns _
@@ -338,15 +338,15 @@ private let take_contains_equiv_exists_helper3 (ty: Type) (s: list ty) (n: nat{n
   )
 
 private let take_contains_equiv_exists_lemma () : Lemma (take_contains_equiv_exists_fact) =
-  introduce forall (ty: Type) (s: seq ty) (n: nat{n <= seq_length s}) (x: ty).
-              seq_contains (seq_take s n) x <==>
-              (exists (i: nat). i < n /\ i < seq_length s /\ seq_index s i == x)
+  introduce forall (ty: Type) (s: seq ty) (n: nat{n <= length s}) (x: ty).
+              contains (take s n) x <==>
+              (exists (i: nat). i < n /\ i < length s /\ index s i == x)
   with (
     take_contains_equiv_exists_helper3 ty s n x
   )
 
 private let rec drop_contains_equiv_exists_helper1 (ty: Type) (s: list ty) (n: nat{n <= length s}) (x: ty)
-  : Lemma (requires memP x (seq_drop s n))
+  : Lemma (requires FLT.memP x (drop s n))
           (ensures (exists (i: nat).{:pattern index s i} n <= i /\ i < length s /\ index s i == x)) =
   match s with
   | hd :: tl ->
@@ -370,12 +370,12 @@ private let rec drop_contains_equiv_exists_helper1 (ty: Type) (s: list ty) (n: n
 
 private let rec drop_contains_equiv_exists_helper2 (ty: Type) (s: list ty) (n: nat{n <= length s}) (x: ty) (i: nat)
   : Lemma (requires (n <= i /\ i < length s /\ index s i == x))
-          (ensures  memP x (seq_drop s n)) =
+          (ensures  FLT.memP x (drop s n)) =
   match s with
   | hd :: tl ->
      eliminate n == 0 \/ n <> 0
-     returns memP x (seq_drop s n)
-     with _. lemma_index_memP s i
+     returns FLT.memP x (drop s n)
+     with _. FLT.lemma_index_memP s i
      and _. (
        drop_contains_equiv_exists_helper2 ty tl (n - 1) x (i - 1);
        eliminate exists (i_tl: nat). n - 1 <= i_tl /\ i_tl < length tl /\ index tl i_tl == x
@@ -384,14 +384,14 @@ private let rec drop_contains_equiv_exists_helper2 (ty: Type) (s: list ty) (n: n
          introduce exists i. n <= i /\ i < length s /\ index s i == x with (i_tl + 1) and ())
 
 private let drop_contains_equiv_exists_helper3 (ty: Type) (s: list ty) (n: nat{n <= length s}) (x: ty)
-  : Lemma (memP x (seq_drop s n) <==>
+  : Lemma (FLT.memP x (drop s n) <==>
            (exists (i: nat).{:pattern index s i} n <= i /\ i < length s /\ index s i == x)) =
-  introduce memP x (seq_drop s n) ==>
+  introduce FLT.memP x (drop s n) ==>
               (exists (i: nat).{:pattern index s i} n <= i /\ i < length s /\ index s i == x)
   with given_antecedent. (
     drop_contains_equiv_exists_helper1 ty s n x);
     introduce (exists (i: nat).{:pattern index s i} n <= i /\ i < length s /\ index s i == x) ==>
-                memP x (seq_drop s n)
+                FLT.memP x (drop s n)
     with given_antecedent. (
       eliminate exists (i: nat). n <= i /\ i < length s /\ index s i == x
       returns _
@@ -400,20 +400,20 @@ private let drop_contains_equiv_exists_helper3 (ty: Type) (s: list ty) (n: nat{n
 
 private let drop_contains_equiv_exists_lemma () : Lemma (drop_contains_equiv_exists_fact) =
   introduce 
-    forall (ty: Type) (s: seq ty) (n: nat{n <= seq_length s}) (x: ty).
-      seq_contains (seq_drop s n) x <==>
-      (exists (i: nat).{:pattern seq_index s i} n <= i /\ i < seq_length s /\ seq_index s i == x)
+    forall (ty: Type) (s: seq ty) (n: nat{n <= length s}) (x: ty).
+      contains (drop s n) x <==>
+      (exists (i: nat).{:pattern index s i} n <= i /\ i < length s /\ index s i == x)
   with (
     drop_contains_equiv_exists_helper3 ty s n x;
-    assert (memP x (seq_drop s n) <==>
-            (exists (i: nat). n <= i /\ i < length s /\ seq_index s i == x))
+    assert (FLT.memP x (drop s n) <==>
+            (exists (i: nat). n <= i /\ i < length s /\ index s i == x))
   )
 
-private let seq_equal_def_lemma () : Lemma (seq_equal_def_fact) =
+private let equal_def_lemma () : Lemma (equal_def_fact) =
   ()
 
-private let seq_extensionality_lemma () : Lemma (seq_extensionality_fact) =
-  introduce forall (ty: Type) (a: seq ty) (b: seq ty). seq_equal a b ==> a == b
+private let extensionality_lemma () : Lemma (extensionality_fact) =
+  introduce forall (ty: Type) (a: seq ty) (b: seq ty). equal a b ==> a == b
   with
     introduce _ ==> _
     with given_antecedent. (
@@ -421,17 +421,17 @@ private let seq_extensionality_lemma () : Lemma (seq_extensionality_fact) =
       with
         introduce _ ==> _
         with given_antecedent. (
-          assert (seq_index a i == seq_index b i) // needed to trigger
+          assert (index a i == index b i) // needed to trigger
         );
       FStar.List.Tot.Properties.index_extensionality a b
     )
 
-private let seq_is_prefix_def_lemma () : Lemma (seq_is_prefix_def_fact) =
+private let is_prefix_def_lemma () : Lemma (is_prefix_def_fact) =
   ()
 
 private let take_length_lemma () : Lemma (take_length_fact) =
   introduce forall (ty: Type) (s: seq ty) (n: nat).
-    n <= seq_length s ==> seq_length (seq_take s n) = n
+    n <= length s ==> length (take s n) = n
   with
     introduce _ ==> _
     with given_antecedent. (
@@ -439,8 +439,8 @@ private let take_length_lemma () : Lemma (take_length_fact) =
     )
 
 private let rec index_into_take_helper (#ty: Type) (s: list ty) (n: nat) (j: nat)
-  : Lemma (requires j < n && n <= length s /\ length (seq_take s n) = n)
-          (ensures  index (seq_take s n) j == index s j) =
+  : Lemma (requires j < n && n <= length s /\ length (take s n) = n)
+          (ensures  index (take s n) j == index s j) =
   match s with
   | hd :: tl -> if j = 0 || n = 0 then () else index_into_take_helper tl (n - 1) (j - 1)
 
@@ -448,26 +448,26 @@ private let index_into_take_lemma ()
   : Lemma (requires take_length_fact) (ensures index_into_take_fact ()) =
   introduce 
     forall (ty: Type) (s: seq ty) (n: nat) (j: nat).
-      j < n && n <= seq_length s ==> seq_index (seq_take s n) j == seq_index s j
+      j < n && n <= length s ==> index (take s n) j == index s j
   with
     introduce _ ==> _
     with given_antecedent. (
-      assert (length (seq_take s n) == n); // triggers take_length_fact
+      assert (length (take s n) == n); // triggers take_length_fact
       index_into_take_helper s n j
     )
 
 private let drop_length_lemma () : Lemma (drop_length_fact) =
   introduce forall (ty: Type) (s: seq ty) (n: nat).
-              n <= seq_length s ==> seq_length (seq_drop s n) = seq_length s - n
+              n <= length s ==> length (drop s n) = length s - n
   with
     introduce _ ==> _
     with given_antecedent. (
-      lemma_splitAt_snd_length n s
+      FLT.lemma_splitAt_snd_length n s
     )
 
 private let rec index_into_drop_helper (#ty: Type) (s: list ty) (n: nat) (j: nat)
-  : Lemma (requires j < length s - n /\ length (seq_drop s n) = length s - n)
-          (ensures  index (seq_drop s n) j == index s (j + n)) =
+  : Lemma (requires j < length s - n /\ length (drop s n) = length s - n)
+          (ensures  index (drop s n) j == index s (j + n)) =
   match s with
   | hd :: tl -> if n = 0 then () else index_into_drop_helper tl (n - 1) j
 
@@ -475,11 +475,11 @@ private let index_into_drop_lemma ()
   : Lemma (requires drop_length_fact) (ensures index_into_drop_fact ()) =
   introduce 
     forall (ty: Type) (s: seq ty) (n: nat) (j: nat).
-      j < seq_length s - n ==> seq_index (seq_drop s n) j == seq_index s (j + n)
+      j < length s - n ==> index (drop s n) j == index s (j + n)
   with
     introduce _ ==> _
     with given_antecedent. (
-      assert (seq_length (seq_drop s n) = seq_length s - n); // triggers drop_length_fact
+      assert (length (drop s n) = length s - n); // triggers drop_length_fact
       index_into_drop_helper s n j
     )
 
@@ -487,17 +487,17 @@ private let drop_index_offset_lemma ()
   : Lemma (requires drop_length_fact) (ensures drop_index_offset_fact ()) =
   introduce 
     forall (ty: Type) (s: seq ty) (n: nat) (k: nat).
-      n <= k && k < seq_length s ==> seq_index (seq_drop s n) (k - n) == seq_index s k
+      n <= k && k < length s ==> index (drop s n) (k - n) == index s k
   with
     introduce _ ==> _
     with given_antecedent. (
-      assert (seq_length (seq_drop s n) = seq_length s - n); // triggers drop_length_fact
+      assert (length (drop s n) = length s - n); // triggers drop_length_fact
       index_into_drop_helper s n (k - n)
     )
 
 private let rec append_then_take_or_drop_helper (#ty: Type) (s: list ty) (t: list ty) (n: nat)
   : Lemma (requires n = length s /\ length (append s t) = length s + length t)
-          (ensures  seq_take (append s t) n == s /\ seq_drop (append s t) n == t) =
+          (ensures  take (append s t) n == s /\ drop (append s t) n == t) =
   match s with
   | [] -> ()
   | hd :: tl -> append_then_take_or_drop_helper tl t (n - 1)
@@ -506,7 +506,7 @@ private let append_then_take_or_drop_lemma ()
   : Lemma (requires append_sums_lengths_fact) (ensures append_then_take_or_drop_fact ()) =
   introduce 
     forall (ty: Type) (s: seq ty) (t: seq ty) (n: nat).
-      n = seq_length s ==> seq_take (seq_append s t) n == s /\ seq_drop (seq_append s t) n == t
+      n = length s ==> take (append s t) n == s /\ drop (append s t) n == t
   with
     introduce _ ==> _
     with given_antecedent. (
@@ -516,9 +516,9 @@ private let append_then_take_or_drop_lemma ()
 private let rec take_commutes_with_in_range_update_helper (#ty: Type) (s: list ty) (i: nat) (v: ty) (n: nat)
   : Lemma (requires   i < n
                     /\ n <= length s
-                    /\ length (seq_update s i v) = length s
-                    /\ length (seq_take s n) = n)
-          (ensures  seq_take (seq_update s i v) n == seq_update (seq_take s n) i v) =
+                    /\ length (update s i v) = length s
+                    /\ length (take s n) = n)
+          (ensures  take (update s i v) n == update (take s n) i v) =
   match s with
   | hd :: tl -> if i = 0 then () else take_commutes_with_in_range_update_helper tl (i - 1) v (n - 1)
 
@@ -527,21 +527,21 @@ private let take_commutes_with_in_range_update_lemma ()
           (ensures take_commutes_with_in_range_update_fact ()) =
   introduce 
     forall (ty: Type) (s: seq ty) (i: nat) (v: ty) (n: nat).
-      i < n && n <= seq_length s ==>
-      seq_take (seq_update s i v) n == seq_update (seq_take s n) i v
+      i < n && n <= length s ==>
+      take (update s i v) n == update (take s n) i v
   with
     introduce _ ==> _
     with given_antecedent. (
-      assert (seq_length (seq_update s i v) = seq_length s); // triggers update_maintains_length_fact
-      assert (seq_length (seq_take s n) = n);                // triggers take_length_fact
+      assert (length (update s i v) = length s); // triggers update_maintains_length_fact
+      assert (length (take s n) = n);            // triggers take_length_fact
       take_commutes_with_in_range_update_helper s i v n
     )
 
 private let rec take_ignores_out_of_range_update_helper (#ty: Type) (s: list ty) (i: nat) (v: ty) (n: nat)
   : Lemma (requires   n <= i
                     /\ i < length s
-                    /\ length (seq_update s i v) = length s)
-          (ensures  seq_take (seq_update s i v) n == seq_take s n) =
+                    /\ length (update s i v) = length s)
+          (ensures  take (update s i v) n == take s n) =
   match s with
   | hd :: tl -> if n = 0 then () else take_ignores_out_of_range_update_helper tl (i - 1) v (n - 1)
 
@@ -550,22 +550,22 @@ private let take_ignores_out_of_range_update_lemma ()
           (ensures take_ignores_out_of_range_update_fact ()) =
   introduce 
     forall (ty: Type) (s: seq ty) (i: nat) (v: ty) (n: nat).
-      n <= i && i < seq_length s ==>
-      seq_take (seq_update s i v) n == seq_take s n
+      n <= i && i < length s ==>
+      take (update s i v) n == take s n
   with
     introduce _ ==> _
     with given_antecedent. (
-      assert (seq_length (seq_update s i v) = seq_length s); // triggers update_maintains_length_fact
+      assert (length (update s i v) = length s); // triggers update_maintains_length_fact
       take_ignores_out_of_range_update_helper s i v n
     )
 
 private let rec drop_commutes_with_in_range_update_helper (#ty: Type) (s: list ty) (i: nat) (v: ty) (n: nat)
   : Lemma (requires   n <= i
                     /\ i < length s
-                    /\ length (seq_update s i v) = length s
-                    /\ length (seq_drop s n) = length s - n)
-          (ensures  seq_drop (seq_update s i v) n ==
-                      seq_update (seq_drop s n) (i - n) v) =
+                    /\ length (update s i v) = length s
+                    /\ length (drop s n) = length s - n)
+          (ensures  drop (update s i v) n ==
+                      update (drop s n) (i - n) v) =
   match s with
   | hd :: tl -> if n = 0 then () else drop_commutes_with_in_range_update_helper tl (i - 1) v (n - 1)
 
@@ -574,21 +574,21 @@ private let drop_commutes_with_in_range_update_lemma ()
           (ensures drop_commutes_with_in_range_update_fact ()) =
   introduce 
     forall (ty: Type) (s: seq ty) (i: nat) (v: ty) (n: nat).
-      n <= i && i < seq_length s ==>
-      seq_drop (seq_update s i v) n == seq_update (seq_drop s n) (i - n) v
+      n <= i && i < length s ==>
+      drop (update s i v) n == update (drop s n) (i - n) v
   with
     introduce _ ==> _
     with given_antecedent. (
-      assert (seq_length (seq_update s i v) = seq_length s); // triggers update_maintains_length_fact
-      assert (seq_length (seq_drop s n) = length s - n);     // triggers drop_length_fact
+      assert (length (update s i v) = length s); // triggers update_maintains_length_fact
+      assert (length (drop s n) = length s - n); // triggers drop_length_fact
       drop_commutes_with_in_range_update_helper s i v n
     )
 
 private let rec drop_ignores_out_of_range_update_helper (#ty: Type) (s: list ty) (i: nat) (v: ty) (n: nat)
   : Lemma (requires   i < n
                     /\ n <= length s
-                    /\ length (seq_update s i v) = length s)
-          (ensures  seq_drop (seq_update s i v) n == seq_drop s n) =
+                    /\ length (update s i v) = length s)
+          (ensures  drop (update s i v) n == drop s n) =
   match s with
   | hd :: tl -> if i = 0 then () else drop_ignores_out_of_range_update_helper tl (i - 1) v (n - 1)
 
@@ -597,18 +597,18 @@ private let drop_ignores_out_of_range_update_lemma ()
           (ensures drop_ignores_out_of_range_update_fact ()) =
   introduce 
     forall (ty: Type) (s: seq ty) (i: nat) (v: ty) (n: nat).
-      i < n && n <= seq_length s ==>
-      seq_drop (seq_update s i v) n == seq_drop s n
+      i < n && n <= length s ==>
+      drop (update s i v) n == drop s n
   with
     introduce _ ==> _
     with given_antecedent. (
-      assert (seq_length (seq_update s i v) = seq_length s); // triggers update_maintains_length_fact
+      assert (length (update s i v) = length s); // triggers update_maintains_length_fact
       drop_ignores_out_of_range_update_helper s i v n
     )
 
 private let rec drop_commutes_with_build_helper (#ty: Type) (s: list ty) (v: ty) (n: nat)
   : Lemma (requires n <= length s /\ length (append s [v]) = 1 + length s)
-          (ensures  seq_drop (append s [v]) n == append (seq_drop s n) [v]) =
+          (ensures  drop (append s [v]) n == append (drop s n) [v]) =
   match s with
   | [] -> ()
   | hd :: tl -> if n = 0 then () else drop_commutes_with_build_helper tl v (n - 1)
@@ -618,37 +618,37 @@ private let drop_commutes_with_build_lemma ()
           (ensures  drop_commutes_with_build_fact ()) =
   introduce 
     forall (ty: Type) (s: seq ty) (v: ty) (n: nat).
-      n <= seq_length s ==> seq_drop (seq_build s v) n == seq_build (seq_drop s n) v
+      n <= length s ==> drop (build s v) n == build (drop s n) v
   with
     introduce _ ==> _
     with given_antecedent. (
-      assert (seq_length (seq_build s v) = 1 + seq_length s); // triggers build_increments_length_fact
+      assert (length (build s v) = 1 + length s); // triggers build_increments_length_fact
       drop_commutes_with_build_helper s v n
     )
 
-private let seq_rank_def_lemma () : Lemma (seq_rank_def_fact) =
+private let rank_def_lemma () : Lemma (rank_def_fact) =
   ()
 
 private let element_ranks_less_lemma () : Lemma (element_ranks_less_fact) =
-  introduce forall (ty: Type) (s: seq ty) (i: nat). i < seq_length s ==> seq_rank (seq_index s i) << seq_rank s
+  introduce forall (ty: Type) (s: seq ty) (i: nat). i < length s ==> rank (index s i) << rank s
   with
     introduce _ ==> _
     with given_antecedent. (
       contains_iff_exists_index_lemma ();
-      assert (seq_contains s (seq_index s i));
-      memP_precedes (seq_index s i) s
+      assert (contains s (index s i));
+      FLT.memP_precedes (index s i) s
     )
 
 private let rec drop_ranks_less_helper (ty: Type) (s: list ty) (i: nat)
   : Lemma (requires 0 < i && i <= length s)
-          (ensures  seq_drop s i << s) =
+          (ensures  drop s i << s) =
   match s with
   | [] -> ()
   | hd :: tl -> if i = 1 then () else drop_ranks_less_helper ty tl (i - 1)
 
 private let drop_ranks_less_lemma () : Lemma (drop_ranks_less_fact) =
   introduce forall (ty: Type) (s: seq ty) (i: nat).
-              0 < i && i <= seq_length s ==> seq_rank (seq_drop s i) << seq_rank s
+              0 < i && i <= length s ==> rank (drop s i) << rank s
   with
     introduce _ ==> _
     with given_antecedent. (
@@ -670,19 +670,19 @@ private let take_zero_lemma () : Lemma (take_zero_fact) =
   ()
 
 private let rec drop_then_drop_helper (#ty: Type) (s: seq ty) (m: nat) (n: nat)
-  : Lemma (requires m + n <= length s /\ length (seq_drop s m) = length s - m)
-          (ensures  seq_drop (seq_drop s m) n == seq_drop s (m + n)) =
+  : Lemma (requires m + n <= length s /\ length (drop s m) = length s - m)
+          (ensures  drop (drop s m) n == drop s (m + n)) =
   match s with
   | [] -> ()
   | hd :: tl -> if m = 0 then () else drop_then_drop_helper tl (m - 1) n
 
 private let drop_then_drop_lemma () : Lemma (requires drop_length_fact) (ensures drop_then_drop_fact ()) =
   introduce forall (ty: Type) (s: seq ty) (m: nat) (n: nat).
-              m + n <= seq_length s ==> seq_drop (seq_drop s m) n == seq_drop s (m + n)
+              m + n <= length s ==> drop (drop s m) n == drop s (m + n)
   with
     introduce _ ==> _
     with given_antecedent. (
-      assert (seq_length (seq_drop s m) = seq_length s - m); // triggers drop_length_fact
+      assert (length (drop s m) = length s - m); // triggers drop_length_fact
       drop_then_drop_helper s m n
     )
 
@@ -706,9 +706,9 @@ let all_dafny_seq_facts_lemma () : Lemma (all_dafny_seq_facts) =
   build_contains_equiv_lemma ();
   take_contains_equiv_exists_lemma ();
   drop_contains_equiv_exists_lemma ();
-  seq_equal_def_lemma ();
-  seq_extensionality_lemma ();
-  seq_is_prefix_def_lemma ();
+  equal_def_lemma ();
+  extensionality_lemma ();
+  is_prefix_def_lemma ();
   take_length_lemma ();
   index_into_take_lemma ();
   drop_length_lemma ();
@@ -720,7 +720,7 @@ let all_dafny_seq_facts_lemma () : Lemma (all_dafny_seq_facts) =
   drop_commutes_with_in_range_update_lemma ();
   drop_ignores_out_of_range_update_lemma ();
   drop_commutes_with_build_lemma ();
-  seq_rank_def_lemma ();
+  rank_def_lemma ();
   element_ranks_less_lemma ();
   drop_ranks_less_lemma ();
   take_ranks_less_lemma ();
