ulib/experimental/FStar.Sequence.Base.fsti
@@ -40,113 +40,112 @@ new val seq (a: Type u#a) : Type u#a
 
 (**
   We translate each Dafny sequence function prefixed with `Seq#`
-  into an F* function prefixed with `seq_`.
+  into an F* function.
 **)
 
-/// We represent the Dafny function `Seq#Length` with `seq_length`:
+/// We represent the Dafny function `Seq#Length` with `length`:
 ///
 /// function Seq#Length<T>(Seq T): int;
 
-val seq_length : #ty: Type -> seq ty -> nat
+val length : #ty: Type -> seq ty -> nat
 
-/// We represent the Dafny function `Seq#Empty` with `seq_empty`:
+/// We represent the Dafny function `Seq#Empty` with `empty`:
 /// 
 /// function Seq#Empty<T>(): Seq T;
 ///
 /// We also provide an alias `nil` for it.
 
-val seq_empty : #ty: Type -> seq ty
-let nil = seq_empty
+val empty : #ty: Type -> seq ty
 
-/// We represent the Dafny function `Seq#Singleton` with `seq_singleton`:
+/// We represent the Dafny function `Seq#Singleton` with `singleton`:
 ///
 /// function Seq#Singleton<T>(T): Seq T;
 
-val seq_singleton : #ty: Type -> ty -> seq ty
+val singleton : #ty: Type -> ty -> seq ty
 
-/// We represent the Dafny function `Seq#Index` with `seq_index`:
+/// We represent the Dafny function `Seq#Index` with `index`:
 ///
 /// function Seq#Index<T>(Seq T, int): T;
 ///
 /// We also provide the infix symbol `$@` for it.
 
-val seq_index: #ty: Type -> s: seq ty -> i: nat{i < seq_length s} -> ty
-let ($@) = seq_index
+val index: #ty: Type -> s: seq ty -> i: nat{i < length s} -> ty
+let ($@) = index
 
-/// We represent the Dafny function `Seq#Build` with `seq_build`:
+/// We represent the Dafny function `Seq#Build` with `build`:
 /// 
 /// function Seq#Build<T>(s: Seq T, val: T): Seq T;
 ///
 /// We also provide the infix symbol `$::` for it.
 
-val seq_build: #ty: Type -> seq ty -> ty -> seq ty
-let ($::) = seq_build
+val build: #ty: Type -> seq ty -> ty -> seq ty
+let ($::) = build
 
-/// We represent the Dafny function `Seq#Append` with `seq_append`:
+/// We represent the Dafny function `Seq#Append` with `append`:
 ///
 /// function Seq#Append<T>(Seq T, Seq T): Seq T;
 ///
 /// We also provide the infix notation `$+` for it.
 
-val seq_append: #ty: Type -> seq ty -> seq ty -> seq ty
-let ($+) = seq_append
+val append: #ty: Type -> seq ty -> seq ty -> seq ty
+let ($+) = append
 
-/// We represent the Dafny function `Seq#Update` with `seq_update`:
+/// We represent the Dafny function `Seq#Update` with `update`:
 ///
 /// function Seq#Update<T>(Seq T, int, T): Seq T;
 
-val seq_update: #ty: Type -> s: seq ty -> i: nat{i < seq_length s} -> ty -> seq ty
+val update: #ty: Type -> s: seq ty -> i: nat{i < length s} -> ty -> seq ty
 
-/// We represent the Dafny function `Seq#Contains` with `seq_contains`:
+/// We represent the Dafny function `Seq#Contains` with `contains`:
 ///
 /// function Seq#Contains<T>(Seq T, T): bool;
 
-val seq_contains: #ty: Type -> seq ty -> ty -> Type0
+val contains: #ty: Type -> seq ty -> ty -> Type0
 
-/// We represent the Dafny function `Seq#Take` with `seq_take`:
+/// We represent the Dafny function `Seq#Take` with `take`:
 ///
 /// function Seq#Take<T>(s: Seq T, howMany: int): Seq T;
 
-val seq_take: #ty: Type -> s: seq ty -> howMany: nat{howMany <= seq_length s} -> seq ty
+val take: #ty: Type -> s: seq ty -> howMany: nat{howMany <= length s} -> seq ty
 
-/// We represent the Dafny function `Seq#Drop` with `seq_drop`:
+/// We represent the Dafny function `Seq#Drop` with `drop`:
 ///
 /// function Seq#Drop<T>(s: Seq T, howMany: int): Seq T;
 
-val seq_drop: #ty: Type -> s: seq ty -> howMany: nat{howMany <= seq_length s} -> seq ty
+val drop: #ty: Type -> s: seq ty -> howMany: nat{howMany <= length s} -> seq ty
 
-/// We represent the Dafny function `Seq#Equal` with `seq_equal`.
+/// We represent the Dafny function `Seq#Equal` with `equal`.
 ///
 /// function Seq#Equal<T>(Seq T, Seq T): bool;
 ///
 /// We also provide the infix symbol `$==` for it.
 
-val seq_equal: #ty: Type -> seq ty -> seq ty -> Type0
-let ($==) = seq_equal
+val equal: #ty: Type -> seq ty -> seq ty -> Type0
+let ($==) = equal
 
 /// Instead of representing the Dafny function `Seq#SameUntil`, which
 /// is only ever used in Dafny to represent prefix relations, we
-/// instead use `seq_is_prefix`.
+/// instead use `is_prefix`.
 ///
 /// function Seq#SameUntil<T>(Seq T, Seq T, int): bool;
 ///
 /// We also provide the infix notation `$<=` for it.
 
-val seq_is_prefix: #ty: Type -> seq ty -> seq ty -> Type0
-let ($<=) = seq_is_prefix
+val is_prefix: #ty: Type -> seq ty -> seq ty -> Type0
+let ($<=) = is_prefix
 
-/// We represent the Dafny function `Seq#Rank` with `seq_rank`.
+/// We represent the Dafny function `Seq#Rank` with `rank`.
 ///
 /// function Seq#Rank<T>(Seq T): int;
 
-val seq_rank: #ty: Type -> ty -> ty
+val rank: #ty: Type -> ty -> ty
 
 (**
   We translate each sequence axiom from the Dafny prelude into an F*
   predicate ending in `_fact`.
 **)
 
-/// We don't need the following axiom since we return a nat from seq_length:
+/// We don't need the following axiom since we return a nat from length:
 /// 
 /// axiom (forall<T> s: Seq T :: { Seq#Length(s) } 0 <= Seq#Length(s));
 
@@ -155,7 +154,7 @@ val seq_rank: #ty: Type -> ty -> ty
 /// axiom (forall<T> :: { Seq#Empty(): Seq T } Seq#Length(Seq#Empty(): Seq T) == 0);
 
 private let length_of_empty_is_zero_fact =
-  forall (ty: Type).{:pattern seq_empty #ty} seq_length (seq_empty #ty) = 0
+  forall (ty: Type).{:pattern empty #ty} length (empty #ty) = 0
 
 /// We represent the following Dafny axiom with `length_zero_implies_empty_fact`:
 ///
@@ -163,14 +162,14 @@ private let length_of_empty_is_zero_fact =
 ///   (Seq#Length(s) == 0 ==> s == Seq#Empty())
 
 private let length_zero_implies_empty_fact =
-  forall (ty: Type) (s: seq ty).{:pattern seq_length s} seq_length s = 0 ==> s == seq_empty
+  forall (ty: Type) (s: seq ty).{:pattern length s} length s = 0 ==> s == empty
 
 /// We represent the following Dafny axiom with `singleton_length_one_fact`:
 /// 
 /// axiom (forall<T> t: T :: { Seq#Length(Seq#Singleton(t)) } Seq#Length(Seq#Singleton(t)) == 1);
 
 private let singleton_length_one_fact =
-  forall (ty: Type) (v: ty).{:pattern seq_length (seq_singleton v)} seq_length (seq_singleton v) = 1
+  forall (ty: Type) (v: ty).{:pattern length (singleton v)} length (singleton v) = 1
 
 /// We represent the following Dafny axiom with `build_increments_length_fact`:
 ///
@@ -179,8 +178,8 @@ private let singleton_length_one_fact =
 ///   Seq#Length(Seq#Build(s,v)) == 1 + Seq#Length(s));
 
 private let build_increments_length_fact =
-  forall (ty: Type) (s: seq ty) (v: ty).{:pattern seq_build s v}
-    seq_length (seq_build s v) = 1 + seq_length s
+  forall (ty: Type) (s: seq ty) (v: ty).{:pattern build s v}
+    length (build s v) = 1 + length s
 
 /// We represent the following Dafny axiom with `index_into_build_fact`:
 ///
@@ -189,10 +188,10 @@ private let build_increments_length_fact =
 ///   (i != Seq#Length(s) ==> Seq#Index(Seq#Build(s,v), i) == Seq#Index(s, i)));
 
 private let index_into_build_fact (_: squash build_increments_length_fact) =
-  forall (ty: Type) (s: seq ty) (v: ty) (i: nat{i < seq_length (seq_build s v)})
-    .{:pattern seq_index (seq_build s v) i}
-      (i = seq_length s ==> seq_index (seq_build s v) i == v)
-    /\ (i <> seq_length s ==> seq_index (seq_build s v) i == seq_index s i)
+  forall (ty: Type) (s: seq ty) (v: ty) (i: nat{i < length (build s v)})
+    .{:pattern index (build s v) i}
+      (i = length s ==> index (build s v) i == v)
+    /\ (i <> length s ==> index (build s v) i == index s i)
 
 /// We represent the following Dafny axiom with `append_sums_lengths_fact`:
 ///
@@ -200,16 +199,16 @@ private let index_into_build_fact (_: squash build_increments_length_fact) =
 ///   Seq#Length(Seq#Append(s0,s1)) == Seq#Length(s0) + Seq#Length(s1));
 
 private let append_sums_lengths_fact =
-  forall (ty: Type) (s0: seq ty) (s1: seq ty).{:pattern seq_length (seq_append s0 s1)}
-    seq_length (seq_append s0 s1) = seq_length s0 + seq_length s1
+  forall (ty: Type) (s0: seq ty) (s1: seq ty).{:pattern length (append s0 s1)}
+    length (append s0 s1) = length s0 + length s1
 
 /// We represent the following Dafny axiom with `index_into_singleton_fact`:
 ///
 /// axiom (forall<T> t: T :: { Seq#Index(Seq#Singleton(t), 0) } Seq#Index(Seq#Singleton(t), 0) == t);
 
 private let index_into_singleton_fact (_: squash singleton_length_one_fact) =
-  forall (ty: Type) (v: ty).{:pattern seq_index (seq_singleton v) 0}
-     seq_index (seq_singleton v) 0 == v
+  forall (ty: Type) (v: ty).{:pattern index (singleton v) 0}
+     index (singleton v) 0 == v
 
 /// We represent the following axiom with `index_after_append_fact`:
 ///
@@ -218,10 +217,10 @@ private let index_into_singleton_fact (_: squash singleton_length_one_fact) =
 ///   (Seq#Length(s0) <= n ==> Seq#Index(Seq#Append(s0,s1), n) == Seq#Index(s1, n - Seq#Length(s0))));
 
 private let index_after_append_fact (_: squash append_sums_lengths_fact) =
-  forall (ty: Type) (s0: seq ty) (s1: seq ty) (n: nat{n < seq_length (seq_append s0 s1)})
-    .{:pattern seq_index (seq_append s0 s1) n}
-      (n < seq_length s0 ==> seq_index (seq_append s0 s1) n == seq_index s0 n)
-    /\ (seq_length s0 <= n ==> seq_index (seq_append s0 s1) n == seq_index s1 (n - seq_length s0))
+  forall (ty: Type) (s0: seq ty) (s1: seq ty) (n: nat{n < length (append s0 s1)})
+    .{:pattern index (append s0 s1) n}
+      (n < length s0 ==> index (append s0 s1) n == index s0 n)
+    /\ (length s0 <= n ==> index (append s0 s1) n == index s1 (n - length s0))
 
 /// We represent the following Dafny axiom with `update_maintains_length`:
 ///
@@ -229,8 +228,8 @@ private let index_after_append_fact (_: squash append_sums_lengths_fact) =
 ///   0 <= i && i < Seq#Length(s) ==> Seq#Length(Seq#Update(s,i,v)) == Seq#Length(s));
 
 private let update_maintains_length_fact =
-  forall (ty: Type) (s: seq ty) (i: nat{i < seq_length s}) (v: ty).{:pattern seq_length (seq_update s i v)}
-    seq_length (seq_update s i v) = seq_length s
+  forall (ty: Type) (s: seq ty) (i: nat{i < length s}) (v: ty).{:pattern length (update s i v)}
+    length (update s i v) = length s
 
 /// We represent the following Dafny axiom with `update_then_index_fact`:
 ///
@@ -240,11 +239,11 @@ private let update_maintains_length_fact =
 ///     (i != n ==> Seq#Index(Seq#Update(s,i,v),n) == Seq#Index(s,n)));
 
 private let update_then_index_fact =
-  forall (ty: Type) (s: seq ty) (i: nat{i < seq_length s}) (v: ty) (n: nat{n < seq_length (seq_update s i v)})
-      .{:pattern seq_index (seq_update s i v) n}
-      n < seq_length s ==>
-          (i = n ==> seq_index (seq_update s i v) n == v)
-        /\ (i <> n ==> seq_index (seq_update s i v) n == seq_index s n)
+  forall (ty: Type) (s: seq ty) (i: nat{i < length s}) (v: ty) (n: nat{n < length (update s i v)})
+      .{:pattern index (update s i v) n}
+      n < length s ==>
+          (i = n ==> index (update s i v) n == v)
+        /\ (i <> n ==> index (update s i v) n == index s n)
 
 /// We represent the following Dafny axiom with `contains_iff_exists_index_fact`:
 ///
@@ -253,8 +252,8 @@ private let update_then_index_fact =
 ///     (exists i: int :: { Seq#Index(s,i) } 0 <= i && i < Seq#Length(s) && Seq#Index(s,i) == x));
 
 private let contains_iff_exists_index_fact =
-  forall (ty: Type) (s: seq ty) (x: ty).{:pattern seq_contains s x}
-    seq_contains s x <==> (exists (i: nat).{:pattern seq_index s i} i < seq_length s /\ seq_index s i == x)
+  forall (ty: Type) (s: seq ty) (x: ty).{:pattern contains s x}
+    contains s x <==> (exists (i: nat).{:pattern index s i} i < length s /\ index s i == x)
 
 /// We represent the following Dafny axiom with `empty_doesnt_contain_fact`:
 ///
@@ -263,7 +262,7 @@ private let contains_iff_exists_index_fact =
 ///   !Seq#Contains(Seq#Empty(), x));
 
 private let empty_doesnt_contain_anything_fact =
-  forall (ty: Type) (x: ty).{:pattern seq_contains seq_empty x} ~(seq_contains seq_empty x)
+  forall (ty: Type) (x: ty).{:pattern contains empty x} ~(contains empty x)
 
 /// We represent the following Dafny axiom with `build_contains_equiv_fact`:
 ///
@@ -272,8 +271,8 @@ private let empty_doesnt_contain_anything_fact =
 ///     Seq#Contains(Seq#Build(s, v), x) <==> (v == x || Seq#Contains(s, x)));
 
 private let build_contains_equiv_fact =
-  forall (ty: Type) (s: seq ty) (v: ty) (x: ty).{:pattern seq_contains (seq_build s v) x}
-    seq_contains (seq_build s v) x <==> (v == x \/ seq_contains s x)
+  forall (ty: Type) (s: seq ty) (v: ty) (x: ty).{:pattern contains (build s v) x}
+    contains (build s v) x <==> (v == x \/ contains s x)
 
 /// We represent the following Dafny axiom with `take_contains_equiv_exists_fact`:
 ///
@@ -284,9 +283,9 @@ private let build_contains_equiv_fact =
 ///       0 <= i && i < n && i < Seq#Length(s) && Seq#Index(s, i) == x));
 
 private let take_contains_equiv_exists_fact =
-  forall (ty: Type) (s: seq ty) (n: nat{n <= seq_length s}) (x: ty).{:pattern seq_contains (seq_take s n) x}
-    seq_contains (seq_take s n) x <==>
-    (exists (i: nat).{:pattern seq_index s i} i < n /\ i < seq_length s /\ seq_index s i == x)
+  forall (ty: Type) (s: seq ty) (n: nat{n <= length s}) (x: ty).{:pattern contains (take s n) x}
+    contains (take s n) x <==>
+    (exists (i: nat).{:pattern index s i} i < n /\ i < length s /\ index s i == x)
 
 /// We represent the following Dafny axiom with `drop_contains_equiv_exists_fact`:
 ///
@@ -297,11 +296,11 @@ private let take_contains_equiv_exists_fact =
 ///       0 <= n && n <= i && i < Seq#Length(s) && Seq#Index(s, i) == x));
 
 private let drop_contains_equiv_exists_fact =
-  forall (ty: Type) (s: seq ty) (n: nat{n <= seq_length s}) (x: ty).{:pattern seq_contains (seq_drop s n) x}
-    seq_contains (seq_drop s n) x <==>
-    (exists (i: nat).{:pattern seq_index s i} n <= i && i < seq_length s /\ seq_index s i == x)
+  forall (ty: Type) (s: seq ty) (n: nat{n <= length s}) (x: ty).{:pattern contains (drop s n) x}
+    contains (drop s n) x <==>
+    (exists (i: nat).{:pattern index s i} n <= i && i < length s /\ index s i == x)
 
-/// We represent the following Dafny axiom with `seq_equal_def_fact`:
+/// We represent the following Dafny axiom with `equal_def_fact`:
 ///
 /// axiom (forall<T> s0: Seq T, s1: Seq T :: { Seq#Equal(s0,s1) }
 ///   Seq#Equal(s0,s1) <==>
@@ -309,24 +308,24 @@ private let drop_contains_equiv_exists_fact =
 ///     (forall j: int :: { Seq#Index(s0,j) } { Seq#Index(s1,j) }
 ///         0 <= j && j < Seq#Length(s0) ==> Seq#Index(s0,j) == Seq#Index(s1,j)));
 
-private let seq_equal_def_fact =
-  forall (ty: Type) (s0: seq ty) (s1: seq ty).{:pattern seq_equal s0 s1}
-    seq_equal s0 s1 <==>
-    seq_length s0 == seq_length s1 /\
-      (forall j.{:pattern seq_index s0 j \/ seq_index s1 j}
-       0 <= j && j < seq_length s0 ==> seq_index s0 j == seq_index s1 j)
+private let equal_def_fact =
+  forall (ty: Type) (s0: seq ty) (s1: seq ty).{:pattern equal s0 s1}
+    equal s0 s1 <==>
+    length s0 == length s1 /\
+      (forall j.{:pattern index s0 j \/ index s1 j}
+       0 <= j && j < length s0 ==> index s0 j == index s1 j)
 
-/// We represent the following Dafny axiom with `seq_extensionality_fact`:
+/// We represent the following Dafny axiom with `extensionality_fact`:
 ///
 /// axiom (forall<T> a: Seq T, b: Seq T :: { Seq#Equal(a,b) }  // extensionality axiom for sequences
 ///   Seq#Equal(a,b) ==> a == b);
 
-private let seq_extensionality_fact =
-  forall (ty: Type) (a: seq ty) (b: seq ty).{:pattern seq_equal a b}
-    seq_equal a b ==> a == b
+private let extensionality_fact =
+  forall (ty: Type) (a: seq ty) (b: seq ty).{:pattern equal a b}
+    equal a b ==> a == b
 
 /// We represent an analog of the following Dafny axiom with
-/// `seq_is_prefix_def_fact`.  Our analog uses `seq_is_prefix` instead
+/// `is_prefix_def_fact`.  Our analog uses `is_prefix` instead
 /// of `Seq#SameUntil`.
 ///
 /// axiom (forall<T> s0: Seq T, s1: Seq T, n: int :: { Seq#SameUntil(s0,s1,n) }
@@ -334,12 +333,12 @@ private let seq_extensionality_fact =
 ///     (forall j: int :: { Seq#Index(s0,j) } { Seq#Index(s1,j) }
 ///         0 <= j && j < n ==> Seq#Index(s0,j) == Seq#Index(s1,j)));
 
-private let seq_is_prefix_def_fact =
-  forall (ty: Type) (s0: seq ty) (s1: seq ty).{:pattern seq_is_prefix s0 s1}
-    seq_is_prefix s0 s1 <==>
-      seq_length s0 <= seq_length s1
-    /\ (forall (j: nat).{:pattern seq_index s0 j \/ seq_index s1 j}
-         j < seq_length s0 ==> seq_index s0 j == seq_index s1 j)
+private let is_prefix_def_fact =
+  forall (ty: Type) (s0: seq ty) (s1: seq ty).{:pattern is_prefix s0 s1}
+    is_prefix s0 s1 <==>
+      length s0 <= length s1
+    /\ (forall (j: nat).{:pattern index s0 j \/ index s1 j}
+         j < length s0 ==> index s0 j == index s1 j)
 
 /// We represent the following Dafny axiom with `take_length_fact`:
 ///
@@ -347,8 +346,8 @@ private let seq_is_prefix_def_fact =
 ///   0 <= n && n <= Seq#Length(s) ==> Seq#Length(Seq#Take(s,n)) == n);
 
 private let take_length_fact =
-  forall (ty: Type) (s: seq ty) (n: nat).{:pattern seq_length (seq_take s n)}
-    n <= seq_length s ==> seq_length (seq_take s n) = n
+  forall (ty: Type) (s: seq ty) (n: nat).{:pattern length (take s n)}
+    n <= length s ==> length (take s n) = n
 
 /// We represent the following Dafny axiom with `index_into_take_fact`.
 ///
@@ -361,8 +360,8 @@ private let take_length_fact =
 
 private let index_into_take_fact (_ : squash take_length_fact) =
   forall (ty: Type) (s: seq ty) (n: nat) (j: nat).
-    {:pattern seq_index (seq_take s n) j \/ seq_index s j ; seq_take s n}
-    j < n && n <= seq_length s ==> seq_index (seq_take s n) j == seq_index s j
+    {:pattern index (take s n) j \/ index s j ; take s n}
+    j < n && n <= length s ==> index (take s n) j == index s j
 
 /// We represent the following Dafny axiom with `drop_length_fact`.
 ///
@@ -371,8 +370,8 @@ private let index_into_take_fact (_ : squash take_length_fact) =
 
 private let drop_length_fact =
   forall (ty: Type) (s: seq ty) (n: nat).
-    {:pattern seq_length (seq_drop s n)}
-    n <= seq_length s ==> seq_length (seq_drop s n) = seq_length s - n
+    {:pattern length (drop s n)}
+    n <= length s ==> length (drop s n) = length s - n
 
 /// We represent the following Dafny axiom with `index_into_drop_fact`.
 ///
@@ -384,8 +383,8 @@ private let drop_length_fact =
 
 private let index_into_drop_fact (_ : squash drop_length_fact) =
   forall (ty: Type) (s: seq ty) (n: nat) (j: nat).
-    {:pattern seq_index (seq_drop s n) j}
-    j < seq_length s - n ==> seq_index (seq_drop s n) j == seq_index s (j + n)
+    {:pattern index (drop s n) j}
+    j < length s - n ==> index (drop s n) j == index s (j + n)
 
 /// We represent the following Dafny axiom with `drop_index_offset_fact`.
 ///
@@ -397,8 +396,8 @@ private let index_into_drop_fact (_ : squash drop_length_fact) =
 
 private let drop_index_offset_fact (_ : squash drop_length_fact) =
   forall (ty: Type) (s: seq ty) (n: nat) (k: nat).
-    {:pattern seq_index s k; seq_drop s n}
-    n <= k && k < seq_length s ==> seq_index (seq_drop s n) (k - n) == seq_index s k
+    {:pattern index s k; drop s n}
+    n <= k && k < length s ==> index (drop s n) (k - n) == index s k
 
 /// We represent the following Dafny axiom with `append_then_take_or_drop_fact`.
 ///
@@ -412,8 +411,8 @@ private let drop_index_offset_fact (_ : squash drop_length_fact) =
 
 private let append_then_take_or_drop_fact (_ : squash append_sums_lengths_fact) =
   forall (ty: Type) (s: seq ty) (t: seq ty) (n: nat).
-    {:pattern seq_take (seq_append s t) n \/ seq_drop (seq_append s t) n}
-    n = seq_length s ==> seq_take (seq_append s t) n == s /\ seq_drop (seq_append s t) n == t
+    {:pattern take (append s t) n \/ drop (append s t) n}
+    n = length s ==> take (append s t) n == s /\ drop (append s t) n == t
 
 /// We represent the following Dafny axiom with `take_commutes_with_in_range_update_fact`.
 ///
@@ -424,9 +423,9 @@ private let append_then_take_or_drop_fact (_ : squash append_sums_lengths_fact) 
 
 private let take_commutes_with_in_range_update_fact
   (_ : squash (update_maintains_length_fact /\ take_length_fact)) =
-  forall (ty: Type) (s: seq ty) (i: nat) (v: ty) (n: nat).{:pattern seq_take (seq_update s i v) n}
-    i < n && n <= seq_length s ==>
-    seq_take (seq_update s i v) n == seq_update (seq_take s n) i v
+  forall (ty: Type) (s: seq ty) (i: nat) (v: ty) (n: nat).{:pattern take (update s i v) n}
+    i < n && n <= length s ==>
+    take (update s i v) n == update (take s n) i v
 
 /// We represent the following Dafny axiom with `take_ignores_out_of_range_update_fact`.
 ///
@@ -435,9 +434,9 @@ private let take_commutes_with_in_range_update_fact
 ///         n <= i && i < Seq#Length(s) ==> Seq#Take(Seq#Update(s, i, v), n) == Seq#Take(s, n));
 
 private let take_ignores_out_of_range_update_fact (_ : squash update_maintains_length_fact) =
-  forall (ty: Type) (s: seq ty) (i: nat) (v: ty) (n: nat).{:pattern seq_take (seq_update s i v) n}
-    n <= i && i < seq_length s ==>
-    seq_take (seq_update s i v) n == seq_take s n
+  forall (ty: Type) (s: seq ty) (i: nat) (v: ty) (n: nat).{:pattern take (update s i v) n}
+    n <= i && i < length s ==>
+    take (update s i v) n == take s n
 
 /// We represent the following Dafny axiom with `drop_commutes_with_in_range_update_fact`.
 ///
@@ -448,9 +447,9 @@ private let take_ignores_out_of_range_update_fact (_ : squash update_maintains_l
 
 private let drop_commutes_with_in_range_update_fact
   (_ : squash (update_maintains_length_fact /\ drop_length_fact)) =
-  forall (ty: Type) (s: seq ty) (i: nat) (v: ty) (n: nat).{:pattern seq_drop (seq_update s i v) n}
-    n <= i && i < seq_length s ==>
-    seq_drop (seq_update s i v) n == seq_update (seq_drop s n) (i - n) v
+  forall (ty: Type) (s: seq ty) (i: nat) (v: ty) (n: nat).{:pattern drop (update s i v) n}
+    n <= i && i < length s ==>
+    drop (update s i v) n == update (drop s n) (i - n) v
 
 /// We represent the following Dafny axiom with `drop_ignores_out_of_range_update_fact`.
 /// Jay noticed that it was unnecessarily weak, possibly due to a typo, so he reported this as
@@ -461,9 +460,9 @@ private let drop_commutes_with_in_range_update_fact
 ///         0 <= i && i < n && n < Seq#Length(s) ==> Seq#Drop(Seq#Update(s, i, v), n) == Seq#Drop(s, n));
 
 private let drop_ignores_out_of_range_update_fact (_ : squash update_maintains_length_fact) =
-  forall (ty: Type) (s: seq ty) (i: nat) (v: ty) (n: nat).{:pattern seq_drop (seq_update s i v) n}
-    i < n && n <= seq_length s ==>
-    seq_drop (seq_update s i v) n == seq_drop s n
+  forall (ty: Type) (s: seq ty) (i: nat) (v: ty) (n: nat).{:pattern drop (update s i v) n}
+    i < n && n <= length s ==>
+    drop (update s i v) n == drop s n
 
 /// We represent the following Dafny axiom with `drop_commutes_with_build_fact`.
 ///
@@ -473,13 +472,13 @@ private let drop_ignores_out_of_range_update_fact (_ : squash update_maintains_l
 ///         Seq#Drop(Seq#Build(s, v), n) == Seq#Build(Seq#Drop(s, n), v) );
 
 private let drop_commutes_with_build_fact (_ : squash build_increments_length_fact) =
-  forall (ty: Type) (s: seq ty) (v: ty) (n: nat).{:pattern seq_drop (seq_build s v) n}
-    n <= seq_length s ==> seq_drop (seq_build s v) n == seq_build (seq_drop s n) v
+  forall (ty: Type) (s: seq ty) (v: ty) (n: nat).{:pattern drop (build s v) n}
+    n <= length s ==> drop (build s v) n == build (drop s n) v
 
-/// We include the definition of `seq_rank` among our facts.
+/// We include the definition of `rank` among our facts.
 
-private let seq_rank_def_fact =
-  forall (ty: Type) (v: ty).{:pattern seq_rank v} seq_rank v == v
+private let rank_def_fact =
+  forall (ty: Type) (v: ty).{:pattern rank v} rank v == v
 
 /// We represent the following Dafny axiom with `element_ranks_less_fact`.
 ///
@@ -488,8 +487,8 @@ private let seq_rank_def_fact =
 ///         0 <= i && i < Seq#Length(s) ==> DtRank($Unbox(Seq#Index(s, i)): DatatypeType) < Seq#Rank(s) );
 
 private let element_ranks_less_fact =
-  forall (ty: Type) (s: seq ty) (i: nat).{:pattern seq_rank (seq_index s i)}
-    i < seq_length s ==> seq_rank (seq_index s i) << seq_rank s
+  forall (ty: Type) (s: seq ty) (i: nat).{:pattern rank (index s i)}
+    i < length s ==> rank (index s i) << rank s
 
 /// We represent the following Dafny axiom with `drop_ranks_less_fact`.
 ///
@@ -498,27 +497,27 @@ private let element_ranks_less_fact =
 ///         0 < i && i <= Seq#Length(s) ==> Seq#Rank(Seq#Drop(s, i)) < Seq#Rank(s) );
 
 private let drop_ranks_less_fact =
-  forall (ty: Type) (s: seq ty) (i: nat).{:pattern seq_rank (seq_drop s i)}
-    0 < i && i <= seq_length s ==> seq_rank (seq_drop s i) << seq_rank s
+  forall (ty: Type) (s: seq ty) (i: nat).{:pattern rank (drop s i)}
+    0 < i && i <= length s ==> rank (drop s i) << rank s
 
 /// We represent the following Dafny axiom with
 /// `take_ranks_less_fact`.  However, since it isn't true in F* (which
-/// has strong requirements for <<), we instead substitute seq_length,
-/// requiring decreases clauses to use seq_length in this case.
+/// has strong requirements for <<), we instead substitute length,
+/// requiring decreases clauses to use length in this case.
 ///
 /// axiom (forall<T> s: Seq T, i: int ::
 ///         { Seq#Rank(Seq#Take(s, i)) }
 ///         0 <= i && i < Seq#Length(s) ==> Seq#Rank(Seq#Take(s, i)) < Seq#Rank(s) );
 
 private let take_ranks_less_fact =
-  forall (ty: Type) (s: seq ty) (i: nat).{:pattern seq_length (seq_take s i)}
-    i < seq_length s ==> seq_length (seq_take s i) << seq_length s
+  forall (ty: Type) (s: seq ty) (i: nat).{:pattern length (take s i)}
+    i < length s ==> length (take s i) << length s
 
 /// We represent the following Dafny axiom with
 /// `append_take_drop_ranks_less_fact`.  However, since it isn't true
 /// in F* (which has strong requirements for <<), we instead
-/// substitute seq_length, requiring decreases clauses to use
-/// seq_length in this case.
+/// substitute length, requiring decreases clauses to use
+/// length in this case.
 ///
 /// axiom (forall<T> s: Seq T, i: int, j: int ::
 ///         { Seq#Rank(Seq#Append(Seq#Take(s, i), Seq#Drop(s, j))) }
@@ -526,8 +525,8 @@ private let take_ranks_less_fact =
 ///         Seq#Rank(Seq#Append(Seq#Take(s, i), Seq#Drop(s, j))) < Seq#Rank(s) );
 
 private let append_take_drop_ranks_less_fact =
-  forall (ty: Type) (s: seq ty) (i: nat) (j: nat).{:pattern seq_length (seq_append (seq_take s i) (seq_drop s j))}
-    i < j && j <= seq_length s ==> seq_length (seq_append (seq_take s i) (seq_drop s j)) << seq_length s
+  forall (ty: Type) (s: seq ty) (i: nat) (j: nat).{:pattern length (append (take s i) (drop s j))}
+    i < j && j <= length s ==> length (append (take s i) (drop s j)) << length s
 
 /// We represent the following Dafny axiom with `drop_zero_fact`.
 ///
@@ -535,8 +534,8 @@ private let append_take_drop_ranks_less_fact =
 ///         n == 0 ==> Seq#Drop(s, n) == s);
 
 private let drop_zero_fact =
-  forall (ty: Type) (s: seq ty) (n: nat).{:pattern seq_drop s n}
-    n = 0 ==> seq_drop s n == s
+  forall (ty: Type) (s: seq ty) (n: nat).{:pattern drop s n}
+    n = 0 ==> drop s n == s
 
 /// We represent the following Dafny axiom with `take_zero_fact`.
 ///
@@ -544,8 +543,8 @@ private let drop_zero_fact =
 ///         n == 0 ==> Seq#Take(s, n) == Seq#Empty());
 
 private let take_zero_fact =
-  forall (ty: Type) (s: seq ty) (n: nat).{:pattern seq_take s n}
-    n = 0 ==> seq_take s n == seq_empty
+  forall (ty: Type) (s: seq ty) (n: nat).{:pattern take s n}
+    n = 0 ==> take s n == empty
 
 /// We represent the following Dafny axiom with `drop_then_drop_fact`.
 ///
@@ -554,8 +553,8 @@ private let take_zero_fact =
 ///         Seq#Drop(Seq#Drop(s, m), n) == Seq#Drop(s, m+n));
 
 private let drop_then_drop_fact (_: squash drop_length_fact) =
-  forall (ty: Type) (s: seq ty) (m: nat) (n: nat).{:pattern seq_drop (seq_drop s m) n}
-    m + n <= seq_length s ==> seq_drop (seq_drop s m) n == seq_drop s (m + n)
+  forall (ty: Type) (s: seq ty) (m: nat) (n: nat).{:pattern drop (drop s m) n}
+    m + n <= length s ==> drop (drop s m) n == drop s (m + n)
 
 (**
   The predicate `all_dafny_seq_facts` collects all the Dafny sequence axioms.
@@ -578,9 +577,9 @@ let all_dafny_seq_facts =
   /\ build_contains_equiv_fact
   /\ take_contains_equiv_exists_fact
   /\ drop_contains_equiv_exists_fact
-  /\ seq_equal_def_fact
-  /\ seq_extensionality_fact
-  /\ seq_is_prefix_def_fact
+  /\ equal_def_fact
+  /\ extensionality_fact
+  /\ is_prefix_def_fact
   /\ take_length_fact
   /\ index_into_take_fact ()
   /\ drop_length_fact
@@ -592,7 +591,7 @@ let all_dafny_seq_facts =
   /\ drop_commutes_with_in_range_update_fact ()
   /\ drop_ignores_out_of_range_update_fact ()
   /\ drop_commutes_with_build_fact ()
-  /\ seq_rank_def_fact
+  /\ rank_def_fact
   /\ element_ranks_less_fact
   /\ drop_ranks_less_fact
   /\ take_ranks_less_fact
